SStructTT/Static/Inversion.lean
@@ -1,7 +1,129 @@
-import SStructTT.Static.Typed
+import SStructTT.Static.Substitution
+open ARS
 
 namespace Static
 variable {Srt : Type} [inst : SStruct Srt]
 
--- lemma Typed.pi_inv {Γ : Ctx Srt} {A B C s} :
---   Γ
+lemma Typed.pi_inv {Γ : Ctx Srt} {A B C r s} :
+    Γ ⊢ .pi A B r s : C ->
+    ∃ sB iB i, A :: Γ ⊢ B : .srt sB iB ∧ C === .srt s i := by
+  generalize e: Tm.pi A B r s = x
+  intro ty; induction ty generalizing A B r s
+  all_goals try trivial
+  case pi sB iA iB _ _ _ _ =>
+    cases e
+    exists sB, iB, (max iA iB)
+    aesop
+  case conv eq1 _ _ ih _ =>
+    have ⟨sB, iB, i, tyB, eq2⟩ := ih e
+    exists sB, iB, i
+    constructor
+    . assumption
+    . apply Conv.trans
+      apply Conv.sym eq1
+      apply eq2
+
+lemma Typed.sig_inv {Γ : Ctx Srt} {A B C r s} :
+    Γ ⊢ .sig A B r s : C ->
+    ∃ sB iB i, A :: Γ ⊢ B : .srt sB iB ∧ C === .srt s i := by
+  generalize e: Tm.sig A B r s = x
+  intro ty; induction ty generalizing A B r s
+  all_goals try trivial
+  case sig sB iA iB _ _ _ _ =>
+    cases e
+    exists sB, iB, (max iA iB)
+    aesop
+  case conv eq1 _ _ ih _ =>
+    have ⟨sB, iB, i, tyB, eq2⟩ := ih e
+    exists sB, iB, i
+    constructor
+    . assumption
+    . apply Conv.trans
+      apply Conv.sym eq1
+      apply eq2
+
+lemma Typed.id_inv {Γ : Ctx Srt} {A B m n} :
+    Γ ⊢ .id A m n : B ->
+    ∃ i, Γ ⊢ m : A ∧ Γ ⊢ n : A ∧ B === .srt s0 i := by
+  generalize e: Tm.id A m n = x
+  intro ty; induction ty generalizing A m n
+  all_goals try trivial
+  case id _ iA _ _ _ _ _ _ =>
+    cases e
+    exists iA
+    aesop
+  case conv eq1 _ _ ih _ =>
+    have ⟨i, tym, tyn, eq2⟩ := ih e
+    exists i
+    and_intros
+    . assumption
+    . assumption
+    . apply Conv.trans
+      apply Conv.sym eq1
+      apply eq2
+
+theorem Typed.valid {Γ : Ctx Srt} {A m} :
+    Γ ⊢ m : A -> ∃ s i, Γ ⊢ A : .srt s i := by
+  intro ty; induction ty
+  all_goals try trivial
+  case srt i _ _ =>
+    exists s0, i+2
+    constructor
+    assumption
+  case var wf hs _ =>
+    have ⟨s, i, _⟩ := wf.has_typed hs
+    exists s, i
+  case pi s _ _ iA iB tyA _ _ _ =>
+    exists s0, (max iA iB + 1)
+    constructor
+    apply tyA.toWf
+  case lam s _ _ _ tym _ ihm =>
+    have wf := tym.toWf
+    cases wf; case cons iA _ _ =>
+    have ⟨_, iB, _⟩ := ihm
+    exists s, (max iA iB)
+    constructor <;> assumption
+  case app ihm _ =>
+    replace ⟨s, i, ihm⟩ := ihm
+    have ⟨s, i, j, tyB, eq⟩ := ihm.pi_inv
+    exists s, i
+    apply Typed.esubst <;> try first | rfl | assumption
+    asimp
+  case sig s _ _ iA iB tyA _ _ _ =>
+    exists s0, (max iA iB + 1)
+    constructor
+    apply tyA.toWf
+  case pair s i _ _ _ _ _ _ =>
+    exists s, i
+  case proj s i _ _ _ _ _ _ =>
+    exists s, i
+    apply Typed.esubst <;> try first | rfl | assumption
+    asimp
+  case bool => exists s0, 1; constructor; assumption
+  case tt => exists s0, 0; constructor; assumption
+  case ff => exists s0, 0; constructor; assumption
+  case ite s i _ _ _ _ _ _ _ _ =>
+    exists s, i
+    apply Typed.esubst <;> try first | rfl | assumption
+    asimp
+  case id i tyA _ _ _ _ _ =>
+    exists s0, i+1; constructor; apply tyA.toWf
+  case rfl ih =>
+    have ⟨s, i, ty⟩ := ih
+    exists s0, i
+    constructor <;> assumption
+  case rw m n a b s i _ _ _ _ _ ihI =>
+    have ⟨sI, iI, tyI⟩ := ihI
+    have ⟨_, tya, tyb, _⟩ := tyI.id_inv
+    exists s, i
+    have : Tm.srt s i = (Tm.srt s i).[n,b/] := by asimp
+    rw[this]
+    apply Typed.substitution
+    . assumption
+    . constructor
+      asimp; assumption
+      constructor
+      asimp; assumption
+      apply AgreeSubst.refl
+      apply tya.toWf
+  case conv => aesop
